\documentclass[11pt,a4paper]{article}
\usepackage[lmargin=1in,rmargin=1in,tmargin=1in,bmargin=1in]{geometry}
\usepackage[pagewise]{lineno} %line numbering
\usepackage{setspace}
\usepackage{ulem} %strikethrough - do not \sout{\cite{}}
\usepackage{xcolor} %change font color
\usepackage{graphicx}
\usepackage{filecontents}
\usepackage{tablefootnote}
\usepackage{footnotehyper}
\usepackage{subfig}
\usepackage[yyyymmdd]{datetime} %date format
\renewcommand{\dateseparator}{.}
\graphicspath{{../img/}} %path to graphics
\setcounter{secnumdepth}{5} %set subsection to nth level
\usepackage{caption}
\captionsetup[table]{skip=11pt} %sets a space after table caption
\usepackage{times}
\usepackage{tabto} %general tabbed spacing
\usepackage{longtable} %need to put label at top under caption then \\ - use spacing
\usepackage[stable,hang,flushmargin]{footmisc} %footnotes in section titles and no indent
\usepackage[round]{natbib} %parenthesis instead of brackets for inline citations
\usepackage{enumitem}
\usepackage{boldline}
\usepackage{makecell}
\usepackage{booktabs}
\usepackage{amssymb}
\usepackage{amsmath}
\usepackage{physics}
\usepackage{tabularx}
\usepackage{multirow}
\usepackage{lscape}
\usepackage{array}
\usepackage{caption}
\usepackage[labelfont=bf]{caption}
\usepackage{chngcntr}
\usepackage{hyperref}

\newcommand{\edit}[1]{\textcolor{blue}{#1}} %shortcut for changing font color on revised text
\newcommand{\fn}[1]{\footnote{#1}} %shortcut for footnote tag
\newcommand*\sq{\mathbin{\vcenter{\hbox{\rule{.3ex}{.3ex}}}}} %makes a small square as a separator $\sq$
\renewcommand\labelenumi{(\theenumi)} %changes 1. to (1) in enumerated list

\usepackage{fancyhdr}
\pagestyle{fancy}
\fancyhf{} %move page number to bottom right
\renewcommand{\headrulewidth}{0.5pt} %turn off line in header
\lhead{\scriptsize NE450 - Principles of nuclear engineering}
\chead{\scriptsize \today}
\rhead{\scriptsize Maxwell equations}
\rfoot{\thepage}

\begin{document}

\begin{titlepage}
    \title{
        NE450 - Principles of nuclear engineering\\
        Maxwell equations\\
    }
    \author{
        R. A. Borrelli
        \\ \\ \\
        University of Idaho $\sq$ Idaho Falls Center for Higher Education
        \\ \\
        Nuclear Engineering and Industrial Management Department
        \\ \\ \\
        r.angelo.borrelli@gmail.com
    }
\clearpage %not have page number on title page
\maketitle
\thispagestyle{empty} %start with page number 1 on second page
\end{titlepage}

\noindent Definition of average energy - 
\begin{equation}
    \overline{E} = \frac{\int_0^{\infty} n(E)EdE}{\int_0^{\infty} n(E)dE}
\end{equation}

\begin{equation}
    n(E) = n_0 \frac{2\pi}{(\pi kT)^{\frac{3}{2}}} \; \sqrt{E} \; e^{-\frac{E}{kT}}
\end{equation}

\noindent Denominator first - 
\begin{equation}
    \int_0^{\infty} n(E)dE \equiv F(E) = a \; n_0 \int_0^{\infty} \sqrt{E} \; e^{-b E} dE 
\end{equation}

\begin{equation*}
    a \equiv \frac{2\pi}{(\pi kT)^{\frac{3}{2}}} 
\end{equation*}

\begin{equation*}
    b \equiv \frac{1}{kT}
\end{equation*}

\begin{equation*}
    \begin{gathered}
        x  = \sqrt{E}\\
        2x \; dx = dE
    \end{gathered}
\end{equation*}

\begin{equation}
    F(E) \rightarrow F(x) = a \; n_0 \int_0^\infty x \; e^{-bx^2} \; 2xdx
\end{equation}

\begin{equation*}
    \int u \; dv = uv - \int v \; du
\end{equation*}

\begin{equation*}
    \begin{gathered}
        u = x\\
        du = dx
    \end{gathered}
\end{equation*}

\begin{equation*}
    \begin{gathered}
        dv = 2x \; e^{-bx^2} \; dx\\
        v = -\frac{1}{b} \; e^{-bx^2}
    \end{gathered}
\end{equation*}

\begin{equation}
    F(x) = a \; n_0 [-\frac{1}{b} \; x \; e^{-bx^2} + \frac{1}{b} \; \int_0^{\infty} e^{-bx^2} \; dx]
\end{equation}

\begin{equation*}
    \begin{gathered}
        w = x\sqrt{b}\\
        \frac{1}{\sqrt{b}} \; dw = dx
    \end{gathered}
\end{equation*}

\begin{equation}
    F(x) = a \; n_0 [-\frac{1}{b} \; x \; e^{-bx^2} + \frac{1}{b} \; \int_0^{\infty} e^{-w^2} \; \frac{1}{b} \; dw]
\end{equation}

\begin{equation}
    F(x) = a \; n_0 [-\frac{1}{b} \; x \; e^{-bx^2} + \frac{1}{b^{\frac{3}{2}}} \; \int_0^{\infty} e^{-w^2} \; dw]
\end{equation}

\begin{equation}
    F(x) = a \; n_0 [-\frac{1}{b} \; x \; e^{-bx^2} + \frac{1}{b^{\frac{3}{2}}} \; \frac{\sqrt{\pi}}{2} \; \int_0^{\infty} \frac{2}{\sqrt{\pi}} \; e^{-w^2} \; dw]
\end{equation}

\begin{equation}
    F(x) = a \; n_0 [-\frac{1}{b} \; x \; e^{-bx^2} + \frac{1}{b^{\frac{3}{2}}} \; \frac{\sqrt{\pi}}{2} \; \erf(w)]
\end{equation}

\begin{equation}
    F(x) = a \; n_0 [-\frac{1}{b} \; x \; e^{-bx^2} + \frac{1}{b^{\frac{3}{2}}} \; \frac{\sqrt{\pi}}{2} \; \erf(x\sqrt{b})]
\end{equation}

\begin{equation}
    F(x) = a \; n_0 \left.[-\frac{1}{b} \; x \; e^{-bx^2} + \frac{1}{b^{\frac{3}{2}}} \; \frac{\sqrt{\pi}}{2} \; \erf(x\sqrt{b})]\right\vert \begin{matrix} \infty \\ 0 \end{matrix}
\end{equation}

\begin{equation}
    F(E) = a \; n_0 \left.[-\frac{1}{b} \; \sqrt{E} \; e^{-bE} + \frac{1}{b^{\frac{3}{2}}} \; \frac{\sqrt{\pi}}{2} \; \erf(\sqrt{bE})]\right\vert \begin{matrix} \infty \\ 0 \end{matrix}
\end{equation}

\begin{equation}
    F(E) = a \; n_0 [(0 + \frac{1}{b^{\frac{3}{2}}} \; \frac{\sqrt{\pi}}{2} \; 1) - (0 + 0)]
\end{equation}

\begin{equation}
    F(E) = \frac{2\pi}{\sqrt{\pi^3 k^3 T^3}} \; n_0 [\frac{k^3 T^3}{} \; \frac{\sqrt{\pi}}{2}]
\end{equation}

\vspace{\baselineskip}

\begin{equation}
    \int_0^{\infty} n(E)dE = n_0
\end{equation}

\newpage

\noindent Now numerator - 
\begin{equation}
    \int_0^{\infty} n(E) E dE \equiv F(E) = a \; n_0 \int_0^{\infty} \sqrt{E} E \; e^{-b E} dE 
\end{equation}

\begin{equation*}
    a \equiv \frac{2\pi}{(\pi kT)^{\frac{3}{2}}} 
\end{equation*}

\begin{equation*}
    b \equiv \frac{1}{kT}
\end{equation*}

\begin{equation*}
    \begin{gathered}
        x  = \sqrt{E}\\
        2x \; dx = dE
    \end{gathered}
\end{equation*}

\begin{equation}
    F(E) \rightarrow F(x) = a \; n_0 \int_0^\infty x \; x^2 \; e^{-bx^2} \; 2xdx
\end{equation}

\begin{equation}
    F(E) \rightarrow F(x) = a \; n_0 \int_0^\infty x^3 \; e^{-bx^2} \; 2xdx
\end{equation}

\begin{equation*}
    \int u \; dv = uv - \int v \; du
\end{equation*}

\begin{equation*}
    \begin{gathered}
        u = x^3\\
        du = 3x^2 \; dx
    \end{gathered}
\end{equation*}

\begin{equation*}
    \begin{gathered}
        dv = 2x \; e^{-bx^2} dx\\
        v = -\frac{1}{b} \; e^{-bx^2}
    \end{gathered}
\end{equation*}

\begin{equation}
    F(x) = a \; n_0 [-\frac{1}{b} x^3 \; e^{-bx^2} + \frac{3}{b} \int_0^{\infty} x^2 \; e^{-bx^2} \; dx]
\end{equation}

\begin{equation}
    F(x) = a \; n_0 [-\frac{1}{b} x^3 \; e^{-bx^2} + \frac{3}{b} (\int_0^{\infty} x \; x \; e^{-bx^2} \; dx)]
\end{equation}

\begin{equation*}
    \begin{gathered}
        u = x\\
        du = dx
    \end{gathered}
\end{equation*}

\begin{equation}
    \begin{gathered}
        dv = x \; e^{-bx^2} \; dx\\
        v = -\frac{1}{2b} \; e^{-bx^2}
    \end{gathered}
\end{equation}

\begin{equation}
    F(x) = a \; n_0 [-\frac{1}{b} \; x^3 \; e^{-bx^2} + \frac{3}{b} (-\frac{1}{2b} \; x \; e^{-bx^2} + \frac{1}{2b} \int_0^{\infty} e^{-bx^2} \; dx)]
\end{equation}

\begin{equation*}
    \begin{gathered}
        w = x\sqrt{b}\\
        \frac{1}{\sqrt{b}} \; dw = dx
    \end{gathered}
\end{equation*}

\begin{equation}
    F(x) = a \; n_0 [-\frac{1}{b} \; x^3 \; e^{-bx^2} + \frac{3}{b} (-\frac{1}{2b} \; x \; e^{-bx^2} + \frac{1}{2b} \int_0^{\infty} e^{-w^2} \; \frac{1}{\sqrt{b}} \; dw)]
\end{equation}

\begin{equation}
    F(x) = a \; n_0 [-\frac{1}{b} \; x^3 \; e^{-bx^2} + \frac{3}{b} (-\frac{1}{2b} \; x \; e^{-bx^2} + \frac{1}{2b^{\frac{3}{2}}} \int_0^{\infty} e^{-w^2} \; dw)]
\end{equation}

\begin{equation}
    F(x) = a \; n_0 [-\frac{1}{b} \; x^3 \; e^{-bx^2} - \frac{3}{2b^2} \; x \; e^{-bx^2} + \frac{3}{2b^{\frac{5}{2}}} \int_0^{\infty} e^{-w^2} \; dw]
\end{equation}

\begin{equation}
    F(x) = a \; n_0 [-\frac{1}{b} \; x^3 \; e^{-bx^2} - \frac{3}{2b^2} \; x \; e^{-bx^2} + \frac{3}{2b^{\frac{5}{2}}} \frac{\sqrt{\pi}}{2} \int_0^{\infty} \frac{2}{\sqrt{\pi}} \; e^{-w^2} \; dw]
\end{equation}

\begin{equation}
    F(x) = a \; n_0 [-\frac{1}{b} \; x^3 \; e^{-bx^2} - \frac{3}{2b^2} \; x \; e^{-bx^2} + \frac{3}{2b^{\frac{5}{2}}} \frac{\sqrt{\pi}}{2} \erf(w)]
\end{equation}

\begin{equation}
    F(x) = a \; n_0 [-\frac{1}{b} \; x^3 \; e^{-bx^2} - \frac{3}{2b^2} \; x \; e^{-bx^2} + \frac{3}{2b^{\frac{5}{2}}} \frac{\sqrt{\pi}}{2} \erf(x\sqrt{b})]
\end{equation}

\begin{equation}
    F(x) = a \; n_0 [-\frac{1}{b} \; \sqrt{E^3} \; e^{-bE} - \frac{3}{2b^2} \; \sqrt{E} \; e^{-bE} + \frac{3}{2b^{\frac{5}{2}}} \frac{\sqrt{\pi}}{2} \erf(\sqrt{bE})]
\end{equation}

\begin{equation}
    F(E) = a \; n_0 \left.[-\frac{1}{b} \; \sqrt{E^3} \; e^{-bE} - \frac{3}{2b^2} \; \sqrt{E} \; e^{-bE} + \frac{3}{2b^{\frac{5}{2}}} \frac{\sqrt{\pi}}{2} \erf(\sqrt{bE})]\right\vert \begin{matrix} \infty \\ 0 \end{matrix}
\end{equation}

\begin{equation}
    F(E) = a \; n_0 [(0 - 0 + \frac{3}{2b^{\frac{5}{2}}} \frac{\sqrt{\pi}}{2}) - (0 - 0 + 0)]
\end{equation}

\begin{equation}
    F(E) = a \; n_0 \; \frac{3}{2b^{\frac{5}{2}}} \frac{\sqrt{\pi}}{2} 
\end{equation}

\begin{equation}
    F(E) = \frac{2\pi}{\sqrt{\pi^3 k^3 T^3}} \; n_0 \; \frac{3\sqrt{k^5 T^5}}{2} \frac{\sqrt{\pi}}{2} 
\end{equation}

\begin{equation}
    F(E) = \frac{}{\sqrt{k^3 T^3}} \; n_0 \; \frac{3\sqrt{k^5 T^5}}{2} 
\end{equation}

\begin{equation}
    F(E) = \frac{3}{2} \; n_0 \; k T 
\end{equation}

\newpage

\begin{equation}
    \overline{E} = \frac{\int_0^{\infty} n(E)EdE}{\int_0^{\infty} n(E)dE}
\end{equation}

\begin{equation}
    \overline{E} = \frac{\frac{3}{2} \; n_0 \; k T}{n_0} 
\end{equation}

\begin{equation}
    \overline{E} = \frac{3}{2} k T 
\end{equation}

\end{document}
